finished initial instantiation, with the last property currently unsatisfied

theories/iris.v
@@ -3,23 +3,19 @@
 
 From mathcomp Require Import ssreflect ssrbool eqtype seq.
 
-From iris.program_logic Require Import language.
+(* There is seemingly a conflict between ssrnat and Iris language. *)
+From iris.program_logic Require Import language ectx_language ectxi_language.
 
 Set Implicit Arguments.
 Unset Strict Implicit.
 Unset Printing Implicit Defensive.
 
-Require Import operations opsem interpreter.
-
-
-Section Host.
-
-Variable host_function : eqType.
+Require Import operations datatypes opsem interpreter binary_format_parser.
 
 Definition expr := host_expr.
 Definition val := host_value.
 Definition state : Type := host_state * store_record * (list host_value).
-Definition observation := unit. (* TODO: maybe change? *)
+Definition observation := unit. (* TODO: ??? *)
 
 Definition of_val (v : val) : expr := HE_value v.
 
@@ -29,83 +25,691 @@ Fixpoint to_val (e : expr) : option val :=
   | _ => None
   end.
 
-Definition prim_step (e : expr) (s : state) (os : list observation) (e' : expr) (s' : state) (fork_es' : list expr) : Prop :=
-  let '(vars, ws, locs) := s in
-  let '(vars', ws', locs') := s' in
-    host_reduce vars ws locs e vars' ws' locs' e' /\ os = [] /\ fork_es' = [].
-
-Lemma to_of_val v : to_val (of_val v) = Some v.
-Proof.
-  by [].
-Qed.
-
 (*
-Definition is_none_or {A : Type} (p : A -> bool) (x : option A) : bool :=
-  match x with
-  | None => true
-  | Some y => p y
-  end.
-
-Lemma to_val_cons_is_none_or_cons : forall e0 e r,
-  to_val (e0 :: e)%SEQ = r -> is_none_or (fun l => l != []) r.
-Proof.
-  move => e0 e.
-  rewrite /=.
-  case.
-  { rewrite /=.
-    case: e0 => //=.
-    case => //=.
-    move => v0 v.
-    case: (to_val e) => //=.
-    move => a H.
-    by case: v H. }
-  { by case: e0. }
-Qed.
+  Identical to host_reduce in opsem.v, but with the 4 rules that are covered in Ectx removed
 *)
+Inductive pure_reduce : host_state -> store_record -> list host_value -> host_expr ->
+                        host_state -> store_record -> list host_value -> host_expr -> Prop :=
+  (* TODO: basic exprs -- arith ops, list ops left *)
+  | pr_getglobal:
+    forall hs s locs id hv,
+      hs id = Some hv ->
+      pure_reduce hs s locs (HE_getglobal id) hs s locs (HE_value hv)
+  | pr_getglobal_trap:
+    forall hs s locs id,
+      hs id = None ->
+      pure_reduce hs s locs (HE_getglobal id) hs s locs (HE_value HV_trap)
+  | pr_setglobal_value:
+    forall hs s locs id hv hs',
+      hv <> HV_trap ->
+      hs' = upd_host_var hs id hv ->
+      pure_reduce hs s locs (HE_setglobal id (HE_value hv)) hs' s locs (HE_value hv)
+  | pr_setglobal_trap:
+    forall hs s locs id,
+      pure_reduce hs s locs (HE_setglobal id (HE_value HV_trap)) hs s locs (HE_value HV_trap)
+  | pr_getlocal:
+    forall hs s locs n hv,
+      List.nth_error locs (nat_of_N n) = Some hv ->
+      pure_reduce hs s locs (HE_getlocal n) hs s locs (HE_value hv)
+  | pr_getlocal_trap:
+    forall hs s locs n,
+      List.nth_error locs (nat_of_N n) = None ->
+      pure_reduce hs s locs (HE_getlocal n) hs s locs (HE_value HV_trap)
+  | pr_setlocal:
+    forall hs s locs n id locs' hv hvd,
+      hs id = Some hv ->
+      (nat_of_N n) < length locs ->
+      locs' = set_nth hvd locs (nat_of_N n) hv ->
+      pure_reduce hs s locs (HE_setlocal n id) hs s locs' (HE_value hv)
+  | pr_setlocal_trap1:
+    forall hs s locs n id,
+      hs id = None ->
+      pure_reduce hs s locs (HE_setlocal n id) hs s locs (HE_value HV_trap)
+  | pr_setlocal_trap2:
+    forall hs s locs n id hv,
+      hs id = Some hv ->
+      (nat_of_N n) >= length locs ->
+      pure_reduce hs s locs (HE_setlocal n id) hs s locs (HE_value HV_trap)
+  | pr_if_true:
+    forall hs s locs id e1 e2 hv,
+      hs id = Some hv ->
+      hv <> HV_wasm_value (VAL_int32 (Wasm_int.int_zero i32m)) ->
+      pure_reduce hs s locs (HE_if id e1 e2) hs s locs e1
+  | pr_if_false: 
+    forall hs s locs id e1 e2 hv,
+      hs id = Some hv ->
+      hv = HV_wasm_value (VAL_int32 (Wasm_int.int_zero i32m)) ->
+      pure_reduce hs s locs (HE_if id e1 e2) hs s locs e2
+  | pr_if_trap: 
+    forall hs s locs id e1 e2,
+      hs id = None ->
+      pure_reduce hs s locs (HE_if id e1 e2) hs s locs (HE_value HV_trap)
+  | pr_while:
+    forall hs s locs id e,
+      pure_reduce hs s locs (HE_while id e) hs s locs (HE_if id (HE_seq e (HE_while id e)) (HE_value (HV_wasm_value (VAL_int32 (Wasm_int.int_zero i32m)))))
+  (* record exprs *)
+  | pr_new_rec:
+    forall hs s locs kip kvp,
+      build_host_kvp hs kip = Some kvp ->
+      pure_reduce hs s locs (HE_new_rec kip) hs s locs (HE_value (HV_record kvp))
+  | pr_new_rec_trap:
+    forall hs s locs kip,
+      build_host_kvp hs kip = None ->
+      pure_reduce hs s locs (HE_new_rec kip) hs s locs (HE_value HV_trap)
+  | pr_getfield:
+    forall hs s locs id fname kvp hv,
+      hs id = Some (HV_record kvp) ->
+      getvalue_kvp kvp fname = Some hv ->
+      pure_reduce hs s locs (HE_get_field id fname) hs s locs (HE_value hv)
+  | pr_getfield_trap1:
+    forall hs s locs id fname kvp,
+      hs id = Some (HV_record kvp) ->
+      getvalue_kvp kvp fname = None ->
+      pure_reduce hs s locs (HE_get_field id fname) hs s locs (HE_value HV_trap)
+  | pr_getfield_trap2:
+    forall hs s locs id fname hv,
+      hs id = Some hv ->
+      host_typeof hv <> Some HT_record ->
+      pure_reduce hs s locs (HE_get_field id fname) hs s locs (HE_value HV_trap)
+  | pr_getfield_trap3:
+    forall hs s locs id fname,
+      hs id = None ->
+      pure_reduce hs s locs (HE_get_field id fname) hs s locs (HE_value HV_trap)
+  (* function exprs *)
+  | pr_new_host_func:
+    forall hs s locs htf locsn e s' n,
+      s' = {|s_funcs := s.(s_funcs) ++ [::FC_func_host htf locsn e]; s_tables := s.(s_tables); s_mems := s.(s_mems); s_globals := s.(s_globals) |} ->
+      n = length s.(s_funcs) ->
+      pure_reduce hs s locs (HE_new_host_func htf (N_of_nat locsn) e) hs s' locs (HE_value (HV_wov (WOV_funcref (Mk_funcidx n))))
+  | pr_call_wasm:
+    forall hs s ids cl id i j vts bes tf vs tn tm vars locs,
+      hs id = Some (HV_wov (WOV_funcref (Mk_funcidx i))) ->
+      List.nth_error s.(s_funcs) i = Some cl ->
+      cl = FC_func_native j tf vts bes ->
+      tf = Tf tn tm ->
+      lookup_host_vars ids hs = Some vars ->
+      list_host_value_to_wasm vars = Some vs ->
+      tn = map typeof vs ->
+      pure_reduce hs s locs (HE_call id ids) hs s locs (HE_wasm_frame ((v_to_e_list vs) ++ [::AI_invoke i]))
+  | pr_call_trap1:
+    forall hs s locs id ids,
+      hs id = None ->
+      pure_reduce hs s locs (HE_call id ids) hs s locs (HE_value HV_trap)
+  | pr_call_trap2:
+    forall hs s locs id ids v,
+      hs id = Some v ->
+      is_funcref v = false ->
+      pure_reduce hs s locs (HE_call id ids) hs s locs (HE_value HV_trap)
+  | pr_call_trap3:
+    forall hs s locs id ids i,
+      hs id = Some (HV_wov (WOV_funcref (Mk_funcidx i))) ->
+      List.nth_error s.(s_funcs) i = None ->
+      pure_reduce hs s locs (HE_call id ids) hs s locs (HE_value HV_trap)  
+  | pr_call_trap4:
+    forall hs s locs id ids,
+      lookup_host_vars ids hs = None ->
+      pure_reduce hs s locs (HE_call id ids) hs s locs (HE_value HV_trap)
+  | pr_call_wasm_trap1:
+    forall hs s locs id ids i cl j tf vts bes vars tn tm,
+      hs id = Some (HV_wov (WOV_funcref (Mk_funcidx i))) ->
+      List.nth_error s.(s_funcs) i = Some cl ->
+      cl = FC_func_native j tf vts bes ->
+      tf = Tf tn tm ->
+      lookup_host_vars ids hs = Some vars ->
+      list_host_value_to_wasm vars = None ->
+      pure_reduce hs s locs (HE_call id ids) hs s locs (HE_value HV_trap)  
+  | pr_call_wasm_trap2:
+    forall hs s locs id ids i cl j tf vts bes vars tn tm vs,
+      hs id = Some (HV_wov (WOV_funcref (Mk_funcidx i))) ->
+      List.nth_error s.(s_funcs) i = Some cl ->
+      cl = FC_func_native j tf vts bes ->
+      tf = Tf tn tm ->
+      lookup_host_vars ids hs = Some vars ->
+      list_host_value_to_wasm vars = Some vs ->
+      tn <> map typeof vs ->
+      pure_reduce hs s locs (HE_call id ids) hs s locs (HE_value HV_trap)  
+  | pr_call_host:
+    forall hs s ids cl id i n e tf tn tm vars vs locs,
+      hs id = Some (HV_wov (WOV_funcref (Mk_funcidx i))) ->
+      List.nth_error s.(s_funcs) i = Some cl ->
+      cl = FC_func_host tf n e ->
+      tf = Tf tn tm ->
+      lookup_host_vars ids hs = Some vars ->
+      list_host_value_to_wasm vars = Some vs -> (* TODO: change this to explicit casts, then add a trap case. *)
+      tn = map typeof vs ->
+      pure_reduce hs s locs (HE_call id ids) hs s locs (HE_wasm_frame ((v_to_e_list vs) ++ [::AI_invoke i]))
+  (* wasm state exprs *)
+  | pr_table_create:
+    forall hs s locs s' tab len n,
+      tab = create_table len ->
+      s' = {|s_funcs := s.(s_funcs); s_tables := s.(s_tables) ++ [::tab]; s_mems := s.(s_mems); s_globals := s.(s_globals) |} ->
+      n = length s.(s_tables) ->
+      pure_reduce hs s locs (HE_wasm_table_create len) hs s' locs (HE_value (HV_wov (WOV_tableref (Mk_tableidx n))))
+  | pr_table_set:
+    forall hs s locs idt n id v tn tab tab' s' tabd fn hvd,
+      hs idt = Some (HV_wov (WOV_tableref (Mk_tableidx tn))) ->
+      List.nth_error s.(s_tables) tn = Some tab ->
+      hs id = Some v ->
+      v = HV_wov (WOV_funcref (Mk_funcidx fn)) ->
+      tab' = {|table_data := set_nth hvd tab.(table_data) n (Some fn); table_max_opt := tab.(table_max_opt) |} ->
+      s' = {|s_funcs := s.(s_funcs); s_tables := set_nth tabd s.(s_tables) tn tab'; s_mems := s.(s_mems); s_globals := s.(s_globals) |} ->
+      pure_reduce hs s locs (HE_wasm_table_set idt (N_of_nat n) id) hs s' locs (HE_value v)
+  | pr_table_get:
+    forall hs s locs idt n tn tab fn,
+      hs idt = Some (HV_wov (WOV_tableref (Mk_tableidx tn))) ->
+      List.nth_error s.(s_tables) tn = Some tab ->
+      List.nth_error tab.(table_data) n = Some (Some fn) ->
+      pure_reduce hs s locs (HE_wasm_table_get idt (N_of_nat n)) hs s locs (HE_value (HV_wov (WOV_funcref (Mk_funcidx fn))))
+  | pr_memory_create:
+    forall hs s locs s' sz sz_lim n,
+      s' = {|s_funcs := s.(s_funcs); s_tables := s.(s_tables); s_mems := s.(s_mems) ++ [::create_memory sz sz_lim]; s_globals := s.(s_globals) |} ->
+      n = length s.(s_mems) ->
+      pure_reduce hs s locs (HE_wasm_memory_create sz sz_lim) hs s' locs (HE_value (HV_wov (WOV_memoryref (Mk_memidx n))))
+  | pr_memory_set:
+    forall hs s locs idm n id mn m m' md' s' memd b,
+      hs idm = Some (HV_wov (WOV_memoryref (Mk_memidx mn))) ->
+      List.nth_error s.(s_mems) mn = Some m ->
+      hs id = Some (HV_byte b) ->
+      memory_list.mem_update n b m.(mem_data) = Some md' ->
+      m' = {|mem_data := md'; mem_max_opt := m.(mem_max_opt) |} ->
+      s' = {|s_funcs := s.(s_funcs); s_tables := s.(s_tables); s_mems := set_nth memd s.(s_mems) mn m'; s_globals := s.(s_globals) |} ->
+      pure_reduce hs s locs (HE_wasm_memory_set idm n id) hs s' locs (HE_value (HV_byte b))
+  | pr_memory_get:
+    forall hs s locs idm n b m mn,
+      hs idm = Some (HV_wov (WOV_memoryref (Mk_memidx mn))) ->
+      List.nth_error s.(s_mems) mn = Some m ->
+      memory_list.mem_lookup n m.(mem_data) = Some b ->
+      pure_reduce hs s locs (HE_wasm_memory_get idm n) hs s locs (HE_value (HV_byte b))
+  | pr_memory_grow:
+    forall hs s s' locs idm n m m' mn memd,
+      hs idm = Some (HV_wov (WOV_memoryref (Mk_memidx mn))) ->
+      List.nth_error s.(s_mems) mn = Some m ->
+      mem_grow m n = Some m' ->
+      s' = {|s_funcs := s.(s_funcs); s_tables := s.(s_tables); s_mems := set_nth memd s.(s_mems) mn m'; s_globals := s.(s_globals) |} ->
+      pure_reduce hs s locs (HE_wasm_memory_grow idm n) hs s' locs (HE_value (HV_wasm_value (VAL_int32 (Wasm_int.int_of_Z i32m (Z.of_N (mem_size m'))))))
+  | pr_globals_create:
+    forall hs s locs s' g n,
+      s' = {|s_funcs := s.(s_funcs); s_tables := s.(s_tables); s_mems := s.(s_mems); s_globals := s.(s_globals) ++ [::g] |} ->
+      n = length s.(s_globals) ->
+      pure_reduce hs s locs (HE_wasm_global_create g) hs s' locs (HE_value (HV_wov (WOV_globalref (Mk_globalidx n))))
+  | pr_global_set:
+    forall hs s locs gn idg id s' v g g' gd,
+      hs id = Some (HV_wasm_value v) ->
+      hs idg = Some (HV_wov (WOV_globalref (Mk_globalidx gn))) ->
+      List.nth_error s.(s_globals) gn = Some g ->
+      g.(g_mut) = MUT_mut ->
+      typeof v = typeof (g.(g_val)) ->
+      g' = {|g_mut := MUT_mut; g_val := v|} ->
+      s' = {|s_funcs := s.(s_funcs); s_tables := s.(s_tables); s_mems := s.(s_mems); s_globals := set_nth gd s.(s_globals) gn g'|} ->
+      pure_reduce hs s locs (HE_wasm_global_set idg id) hs s' locs (HE_value (HV_wasm_value v))
+  | pr_global_get:
+    forall hs s locs idg g gn v,
+      hs idg = Some (HV_wov (WOV_globalref (Mk_globalidx gn))) ->
+      g.(g_val) = v ->
+      pure_reduce hs s locs (HE_wasm_global_get idg) hs s locs (HE_value (HV_wasm_value v))
+  (* wasm module expr *)
+  | pr_compile:
+    forall hs s locs id mo hvl hbytes,
+      hs id = Some (HV_list hvl) ->
+      to_bytelist hvl = Some hbytes ->
+      run_parse_module (map byte_of_compcert_byte hbytes) = Some mo -> (* Check: is this correct? *)
+      pure_reduce hs s locs (HE_compile id) hs s locs (HE_value (HV_module mo))
+  (* TODO: replace the proxy *)
+  | pr_instantiate:
+    forall hs s locs idm idr mo r rec,
+      hs idm = Some (HV_module mo) ->
+      hs idr = Some (HV_record r) ->
+      pure_reduce hs s locs (HE_instantiate idm idr) hs s locs rec
+  (* miscellaneous *)
+  | pr_seq_const:
+    forall hs s locs v e,
+      pure_reduce hs s locs (HE_seq (HE_value v) e) hs s locs e
+  | pr_wasm_return:
+    forall hs s locs vs,      
+      pure_reduce hs s locs (HE_wasm_frame (v_to_e_list vs)) hs s locs (HE_value (HV_list (map (fun wv => (HV_wasm_value wv)) vs)))
+  | pr_wasm_return_trap:
+      forall hs s locs,
+      pure_reduce hs s locs (HE_wasm_frame ([::AI_trap])) hs s locs (HE_value (HV_trap))
+  | pr_host_return:
+    forall hs s locsf locs ids e vs tn,
+      lookup_host_vars ids hs = Some vs ->
+      pure_reduce hs s locsf (HE_host_frame tn locs (HE_seq (HE_return ids) e)) hs s locsf (HE_value (HV_list vs))
+   
+
+(* TODO: needs all the host_expr reduction steps: compile, instantiate, etc. *)
+(* TODO: needs restructuring to make sense *)
+with wasm_reduce : host_state -> store_record -> frame -> list administrative_instruction ->
+                   host_state -> store_record -> frame -> list administrative_instruction -> Prop :=
+  | wr_simple :
+      forall e e' s f hs,
+        reduce_simple e e' ->
+        wasm_reduce hs s f e hs s f e'
+
+  (** calling operations **)
+  | wr_call :
+      forall s f i a hs,
+        List.nth_error f.(f_inst).(inst_funcs) i = Some a ->
+        wasm_reduce hs s f [::AI_basic (BI_call i)] hs s f [::AI_invoke a]
+  | wr_call_indirect_success :
+      forall s f i a cl tf c hs,
+        stab_addr s f (Wasm_int.nat_of_uint i32m c) = Some a ->
+        List.nth_error s.(s_funcs) a = Some cl ->
+        cl_type cl = Some tf ->
+        stypes s f.(f_inst) i = Some tf ->
+        wasm_reduce hs s f [::AI_basic (BI_const (VAL_int32 c)); AI_basic (BI_call_indirect i)] hs s f [::AI_invoke a]
+  | wr_call_indirect_failure1 :
+      forall s f i a cl tf c hs,
+        stab_addr s f (Wasm_int.nat_of_uint i32m c) = Some a ->
+        List.nth_error s.(s_funcs) a = Some cl ->
+        cl_type cl = Some tf ->
+        stypes s f.(f_inst) i <> Some tf ->
+        wasm_reduce hs s f [::AI_basic (BI_const (VAL_int32 c)); AI_basic (BI_call_indirect i)] hs s f [::AI_trap]
+  | wr_call_indirect_failure2 :
+      forall s f i c hs,
+        stab_addr s f (Wasm_int.nat_of_uint i32m c) = None ->
+        wasm_reduce hs s f [::AI_basic (BI_const (VAL_int32 c)); AI_basic (BI_call_indirect i)] hs s f [::AI_trap]
+  | wr_invoke_native :
+      forall a cl t1s t2s ts es ves vcs n m k zs s f f' i hs,
+        List.nth_error s.(s_funcs) a = Some cl ->
+        cl = FC_func_native i (Tf t1s t2s) ts es ->
+        ves = v_to_e_list vcs ->
+        length vcs = n ->
+        length ts = k ->
+        length t1s = n ->
+        length t2s = m ->
+        n_zeros ts = zs ->
+        f'.(f_inst) = i ->
+        f'.(f_locs) = vcs ++ zs ->
+        wasm_reduce hs s f (ves ++ [::AI_invoke a]) hs s f [::AI_local m f' [::AI_basic (BI_block (Tf [::] t2s) es)]]
+  | wr_invoke_host :
+    (* TODO: check *)
+    (* TODO: check - R *)  
+    forall a cl e tf t1s t2s ves vcs m n s s' f hs hs' vs,
+      List.nth_error s.(s_funcs) a = Some cl ->
+      cl = FC_func_host tf n e ->
+      tf = Tf t1s t2s ->
+      ves = v_to_e_list vcs ->
+      length vcs = n ->
+      length t1s = n ->
+      length t2s = m ->
+      Some vs = lookup_host_vars_as_i32s vcs hs ->
+      wasm_reduce hs s f (ves ++ [::AI_invoke a]) hs' s' f [::AI_host_frame t1s vs e]
+
+  | wr_host_step :
+    (* TODO: check *)
+    forall hs s (f : frame) ts vs e hs' s' vs' e',
+      pure_reduce hs s vs e hs' s' vs' e' ->
+        wasm_reduce hs s f [::AI_host_frame ts vs e] hs' s' f [::AI_host_frame ts vs' e']
+  | wr_host_return :
+    (* TODO: check *)
+    forall hs s f ts vs ids vs' vs'',
+    Some vs' = lookup_host_vars ids hs ->
+    Some vs'' = list_extra.those (List.map (fun x => match x with | HV_wasm_value v => Some v | _ => None end) vs') ->
+    wasm_reduce hs s f [::AI_host_frame ts vs (HE_return ids)] hs s f (v_to_e_list vs'')
+(*  
+  | wr_host_new_host_func :
+    (* TODO: check *)
+    forall hs s f ts vs tf n e idx idx_h hs' s',
+    idx = List.length s.(s_funcs) ->
+    idx_h = List.length hs.(hs_funcs) ->
+    hs' = {| hs_varmap := hs.(hs_varmap); hs_funcs := hs.(hs_funcs) ++ [::e] |} ->
+    s' = {| s_funcs := s.(s_funcs) ++ [::(FC_func_host tf (Mk_funcidx idx_h))]; s_tables := s.(s_tables); s_mems := s.(s_mems); s_globals := s.(s_globals) |} ->
+    wasm_reduce hs s f [::AI_host_frame ts vs (HE_new_host_func tf n e)]
+      hs' s' f [::AI_host_frame ts vs (HE_value (HV_wov (WOV_funcref (Mk_funcidx idx_h))))]
+*)
+  (** get, set, load, and store operations **)
+  | wr_get_local :
+      forall f v j s hs,
+        List.nth_error f.(f_locs) j = Some v ->
+        wasm_reduce hs s f [::AI_basic (BI_get_local j)] hs s f [::AI_basic (BI_const v)]
+  | wr_set_local :
+      forall f f' i v s vd hs,
+        f'.(f_inst) = f.(f_inst) ->
+        f'.(f_locs) = set_nth vd f.(f_locs) i v ->
+        wasm_reduce hs s f [::AI_basic (BI_const v); AI_basic (BI_set_local i)] hs s f' [::]
+  | wr_get_global :
+      forall s f i v hs,
+        sglob_val s f.(f_inst) i = Some v ->
+        wasm_reduce hs s f [::AI_basic (BI_get_global i)] hs s f [::AI_basic (BI_const v)]
+  | wr_set_global :
+      forall s f i v s' hs,
+        supdate_glob s f.(f_inst) i v = Some s' ->
+        wasm_reduce hs s f [::AI_basic (BI_const v); AI_basic (BI_set_global i)] hs s' f [::]
+  | wr_load_success :
+    forall s i f t bs k a off m hs,
+      smem_ind s f.(f_inst) = Some i ->
+      List.nth_error s.(s_mems) i = Some m ->
+      load m (Wasm_int.N_of_uint i32m k) off (t_length t) = Some bs ->
+      wasm_reduce hs s f [::AI_basic (BI_const (VAL_int32 k)); AI_basic (BI_load t None a off)] hs s f [::AI_basic (BI_const (wasm_deserialise bs t))]
+  | wr_load_failure :
+    forall s i f t k a off m hs,
+      smem_ind s f.(f_inst) = Some i ->
+      List.nth_error s.(s_mems) i = Some m ->
+      load m (Wasm_int.N_of_uint i32m k) off (t_length t) = None ->
+      wasm_reduce hs s f [::AI_basic (BI_const (VAL_int32 k)); AI_basic (BI_load t None a off)] hs s f [::AI_trap]
+  | wr_load_packed_success :
+    forall s i f t tp k a off m bs sx hs,
+      smem_ind s f.(f_inst) = Some i ->
+      List.nth_error s.(s_mems) i = Some m ->
+      load_packed sx m (Wasm_int.N_of_uint i32m k) off (tp_length tp) (t_length t) = Some bs ->
+      wasm_reduce hs s f [::AI_basic (BI_const (VAL_int32 k)); AI_basic (BI_load t (Some (tp, sx)) a off)] hs s f [::AI_basic (BI_const (wasm_deserialise bs t))]
+  | wr_load_packed_failure :
+    forall s i f t tp k a off m sx hs,
+      smem_ind s f.(f_inst) = Some i ->
+      List.nth_error s.(s_mems) i = Some m ->
+      load_packed sx m (Wasm_int.N_of_uint i32m k) off (tp_length tp) (t_length t) = None ->
+      wasm_reduce hs s f [::AI_basic (BI_const (VAL_int32 k)); AI_basic (BI_load t (Some (tp, sx)) a off)] hs s f [::AI_trap]
+  | wr_store_success :
+    forall t v s i f mem' k a off m hs,
+      types_agree t v ->
+      smem_ind s f.(f_inst) = Some i ->
+      List.nth_error s.(s_mems) i = Some m ->
+      store m (Wasm_int.N_of_uint i32m k) off (bits v) (t_length t) = Some mem' ->
+      wasm_reduce hs s f [::AI_basic (BI_const (VAL_int32 k)); AI_basic (BI_const v); AI_basic (BI_store t None a off)] hs (upd_s_mem s (update_list_at s.(s_mems) i mem')) f [::]
+  | wr_store_failure :
+    forall t v s i f m k off a hs,
+      types_agree t v ->
+      smem_ind s f.(f_inst) = Some i ->
+      List.nth_error s.(s_mems) i = Some m ->
+      store m (Wasm_int.N_of_uint i32m k) off (bits v) (t_length t) = None ->
+      wasm_reduce hs s f [::AI_basic (BI_const (VAL_int32 k)); AI_basic (BI_const v); AI_basic (BI_store t None a off)] hs s f [::AI_trap]
+  | wr_store_packed_success :
+    forall t v s i f m k off a mem' tp hs,
+      types_agree t v ->
+      smem_ind s f.(f_inst) = Some i ->
+      List.nth_error s.(s_mems) i = Some m ->
+      store_packed m (Wasm_int.N_of_uint i32m k) off (bits v) (tp_length tp) = Some mem' ->
+      wasm_reduce hs s f [::AI_basic (BI_const (VAL_int32 k)); AI_basic (BI_const v); AI_basic (BI_store t (Some tp) a off)] hs (upd_s_mem s (update_list_at s.(s_mems) i mem')) f [::]
+  | wr_store_packed_failure :
+    forall t v s i f m k off a tp hs,
+      types_agree t v ->
+      smem_ind s f.(f_inst) = Some i ->
+      List.nth_error s.(s_mems) i = Some m ->
+      store_packed m (Wasm_int.N_of_uint i32m k) off (bits v) (tp_length tp) = None ->
+      wasm_reduce hs s f [::AI_basic (BI_const (VAL_int32 k)); AI_basic (BI_const v); AI_basic (BI_store t (Some tp) a off)] hs s f [::AI_trap]
+
+  (** memory **)
+  | wr_current_memory :
+      forall i f m n s hs,
+        smem_ind s f.(f_inst) = Some i ->
+        List.nth_error s.(s_mems) i = Some m ->
+        mem_size m = n ->
+        wasm_reduce hs s f [::AI_basic (BI_current_memory)] hs s f [::AI_basic (BI_const (VAL_int32 (Wasm_int.int_of_Z i32m (Z.of_N n))))]
+  | wr_grow_memory_success :
+    forall s i f m n mem' c hs,
+      smem_ind s f.(f_inst) = Some i ->
+      List.nth_error s.(s_mems) i = Some m ->
+      mem_size m = n ->
+      mem_grow m (Wasm_int.N_of_uint i32m c) = Some mem' ->
+      wasm_reduce hs s f [::AI_basic (BI_const (VAL_int32 c)); AI_basic BI_grow_memory] hs (upd_s_mem s (update_list_at s.(s_mems) i mem')) f [::AI_basic (BI_const (VAL_int32 (Wasm_int.int_of_Z i32m (Z.of_N n))))]
+  | wr_grow_memory_failure :
+      forall i f m n s c hs,
+        smem_ind s f.(f_inst) = Some i ->
+        List.nth_error s.(s_mems) i = Some m ->
+        mem_size m = n ->
+        wasm_reduce hs s f [::AI_basic (BI_const (VAL_int32 c)); AI_basic BI_grow_memory] hs s f [::AI_basic (BI_const (VAL_int32 int32_minus_one))]
+
+  (** label and local **)
+  | wr_label :
+      forall s f es les s' f' es' les' k lh hs hs',
+        wasm_reduce hs s f es hs' s' f' es' ->
+        lfilled k lh es les ->
+        lfilled k lh es' les' ->
+        wasm_reduce hs s f les hs' s' f' les'
+  | wr_local :
+      forall s f es s' f' es' n f0 hs hs',
+        wasm_reduce hs s f es hs' s' f' es' ->
+        wasm_reduce hs s f0 [::AI_local n f es] hs' s' f0 [::AI_local n f' es']
+.
+
+
+Inductive head_reduce: state -> expr -> state -> expr -> Prop :=
+  | purer_headr:
+    forall hs s locs e hs' s' locs' e',
+      pure_reduce hs s locs e hs' s' locs' e' ->
+      head_reduce (hs, s, locs) e (hs', s', locs') e'.
+
+ Definition head_step (e : expr) (s : state) (os : list observation) (e' : expr) (s' : state) (es' : list expr) : Prop :=
+  head_reduce s e s' e' /\
+  os = nil /\
+  es' = nil. (* ?? *) 
+
 Lemma of_to_val e v : to_val e = Some v → of_val v = e.
 Proof.
   destruct e => //=.
   move => H. by inversion H.
 Qed.
 
-Lemma val_head_stuck : forall e1 s1 κ e2 s2 efs,
-  prim_step e1 s1 κ e2 s2 efs →
-  to_val e1 = None.
-Proof.
-(*
-  rewrite /prim_step => e1 [hs1 σ1] κ e2 [hs2 σ2] efs.
-  case_eq (split_vals_e e1) => vs es H.
-  case_eq (split_vals_e e2) => vs' es' _ [i [Hred _]].
-  move: vs vs' es' H Hred.
-  elim: es.
-  { move => vs vs' es' _ Hred.
-    exfalso.
-    apply: reduce_not_nil.
-    apply: Hred.
-    done. }
-  { move => e es _ vs vs' _ H1 _ {e2 efs}.
-    apply: splits_vals_e_to_val_hd.
-    apply: H1. }*)
-Admitted.
-
-Inductive ectx_item := (* what items do we need??? *)
-  (* Host/Wasm frame. But do we need the Label case in Wasm as well?? *)
+Inductive ectx_item := (* what items do we need exactly? *)
+  (* Host/Wasm frame. But do we need the Label case in Wasm to be here as well?? *)
 | Ectx_setglobal : id -> ectx_item
-| Ectx_seq : expr -> ectx_item.
+| Ectx_seq : expr -> ectx_item
+(*| Ectx_wasm_frame: list administrative_instruction -> ectx_item*)
+| Ectx_host_frame: list value_type -> list host_value -> ectx_item
+.
 
-Fixpoint fill_item (Ki : ectx_item) (e : expr) : expr :=
+Definition fill_item (Ki : ectx_item) (e : expr) : expr :=
   match Ki with
   | Ectx_setglobal id => HE_setglobal id e
   | Ectx_seq e' => HE_seq e' e
+  (* There's currently a problem with this one -- the expression within context, we, is not
+     a general expression of type expr. Maybe this should not be a context? 
+  | Ectx_wasm_frame we => HE_wasm_frame we*)
+  | Ectx_host_frame tf locs => HE_host_frame tf locs e
   end.
 
-(* Need to be in Ectxilanguagemixin. But what is the diff between head_step and prim_step? *)
-Lemma wasm_mixin : LanguageMixin of_val to_val prim_step.
-Proof. split; eauto using to_of_val, of_to_val, val_head_stuck. Qed.
+Lemma head_step_not_val: forall e1 σ1 κ e2 σ2 efs,
+  head_step e1 σ1 κ e2 σ2 efs ->
+  to_val e1 = None.
+Proof.
+  move => e1 σ1 κ e2 σ2 efs H.
+  destruct H as [HR _].
+  inversion HR as [hs s locs e hs' s' locs' e' H]; subst.
+  by inversion H.
+Qed.
+
+Lemma fill_val: forall Ki e,
+  is_Some (to_val (fill_item Ki e)) -> is_Some (to_val e).
+Proof.
+  move => Ki e H.
+  destruct H as [v He].
+  by destruct Ki; inversion He.
+Qed.
+  
+Lemma fill_inj: forall Ki,
+  Inj eq eq (fill_item Ki).
+Proof.
+  unfold Inj.
+  move => Ki x y Himage.
+  by destruct Ki; inversion Himage.
+Qed.
+
+Lemma fill_expr_inj: forall Ki1 Ki2 e1 e2,
+  to_val e1 = None ->
+  to_val e2 = None ->
+  fill_item Ki1 e1 = fill_item Ki2 e2 ->
+  Ki1 = Ki2.
+Proof.
+  move => Ki1 Ki2 e1 e2 Hv1 Hv2 Himage.
+  by destruct Ki1; destruct Ki2; inversion Himage.
+Qed.
+
+(* For this one to hold, all the reductions related to propagating within evaluation contexts
+     needs to be removed from head_step. 
+   However, note that this is currently not true with how we want to return from a host frame:
+     we require an explicit instruction HE_return to return from the context, while this property
+     seems to require that the only case where evaluation contexts could be further reduced
+     should be the case where the expression in the context is already a value.
+   Another rule that violates this property is the reduction of (SEQ v e) -> e. Is this already
+     included in how Iris deals with evaluation contexts, though? If yes then there's no problem.
+*)
+Lemma head_step_return_val: forall Ki e σ1 κ e2 σ2 efs,
+  head_step (fill_item Ki e) σ1 κ e2 σ2 efs ->
+  is_Some (to_val e).
+Proof.
+  move => Ki e σ1 κ e2 σ2 efs H.
+  destruct H as [HR _].
+  inversion HR as [hs s locs e0 hs' s' locs' e0' H]; subst. clear HR.
+  destruct Ki; simpl in H; inversion H; subst => //=; try by eauto.
+Admitted.
+  
+Lemma wasm_mixin : EctxiLanguageMixin of_val to_val fill_item head_step.
+Proof.
+  split => //.
+  - by apply of_to_val.
+  - by apply head_step_not_val.
+  - by apply fill_val.
+  - by apply fill_inj.
+  - by apply fill_expr_inj.
+  - by apply head_step_return_val. (* This one is currently not true. *)
+  
+  (* So seems like this is what we need to do:
+     - Define the values/expressions of the language, and the conversions (of_val, to_val);
+     - Define the evaluation contexts (extx_item, fill_item);
+     - Define the opsem of the language, but this is now without the cases for evaluation 
+         contexts (because Iris want to handle those separately? )
+     - Prove that what we defined above for this EctxiLanguagemixin 
+         satisfy certain properties (7 of them here, seemingly). *)
+Admitted.
+
+Canonical Structure wasm_ectxi_lang := EctxiLanguage wasm_mixin.
+Canonical Structure wasm_ectx_lang := EctxLanguageOfEctxi wasm_ectxi_lang.
+Canonical Structure wasm_lang := LanguageOfEctx wasm_ectx_lang.
+
+
+(* Copied without thoughts. But it looks like we need to prove a spec for each reduction
+     (like a triple for each reduction ). *)
+
+From stdpp Require Import fin_maps.
+From iris.proofmode Require Import tactics.
+From iris.algebra Require Import auth gmap.
+From iris.bi.lib Require Import fractional.
+From iris.base_logic.lib Require Export gen_heap proph_map.
+From iris.program_logic Require Export weakestpre total_weakestpre.
+From iris.program_logic Require Import ectx_lifting total_ectx_lifting.
+
+
+From iris.heap_lang Require Import locations.
+
+Definition proph_id := unit. (* ??? *)
+
+Class heapG Σ := HeapG {
+  heapG_invG : invG Σ;
+  heapG_gen_heapG :> gen_heapG loc (option val) Σ;
+  heapG_proph_mapG :> proph_mapG proph_id (val * val) Σ;
+}.
 
 (*
-Lemma wasm_mixin : EctxiLanguageMixin of_val to_val fill_item head_step.
-*)  
+(* TODO: this is a dummy definition that only takes globals into account *)
+Definition pmap_of_store_record (σ : store_record) : pmap.Pmap (option val).
+refine (list_extra.fold_lefti _ σ.(s_globals) _).
+{ move => i pm glob.
+  apply: pmap.Pmerge.
+  apply: (fun x y =>
+    match (x, y) with
+    | (None, None) => None
+    | (Some xx, _) => Some xx
+    | (_, Some yy) => Some yy
+    end).
+  apply: pm.
+  pose v := Some (cons glob.(g_val) nil).
+  refine (@pmap.PMap _ (@pmap.Psingleton_raw _ (Pos.of_succ_nat i) v) _).
+  apply: pmap.Psingleton_wf.
+}
+{ apply: pmap.Pempty. }
+Defined.
 
-End Host.
+Definition gmap_of_store_record (σ : store_record) : gmap loc (option val) :=
+  list_extra.fold_lefti
+    (λ (i : nat) (pm : gmap loc (option val)) (glob : global),
+       map_insert {| loc_car := Z.of_nat i |} (Some [g_val glob]) pm)
+    (s_globals σ) ∅.
+
+Instance heapG_irisG `{!heapG Σ} : irisG wasm_lang Σ := {
+  iris_invG := heapG_invG;
+  state_interp σ κs _ :=
+    gen_heap_ctx (gmap_of_store_record σ);
+  fork_post z := True%I;
+}.
+
+Notation "l ↦{ q } v" := (mapsto (L:=loc) (V:=option val) l q (Some v%V))
+  (at level 20, q at level 50, format "l  ↦{ q }  v") : bi_scope.
+
+  Ltac inv_head_step :=
+    repeat match goal with
+    | _ => progress simplify_map_eq/= (* simplify memory stuff *)
+    | H : to_val _ = Some _ |- _ => apply of_to_val in H
+    | H : head_step ?e _ _ _ _ _ |- _ =>
+       try (is_var e; fail 1); (* inversion yields many goals if [e] is a variable
+       and can thus better be avoided. *)
+       inversion H; subst; clear H
+    end.
+  
+
+Definition locof (n : nat) := {| loc_car := (Z.of_nat n) |}.
+
+Section lifting.
+Context `{!heapG Σ}.
+Implicit Types σ : state.
+
+Lemma twp_load s E imm q v :
+  [[{ (locof imm) ↦{q} v }]] [Basic (Get_local imm)] @ s; E [[{ RET v; (locof imm) ↦{q} v }]].
+Proof.
+  iIntros (Φ) "Hl HΦ". iApply twp_lift_atomic_head_step_no_fork; first done.
+  iIntros (σ1 κs n) "Hσ !>". iDestruct (@gen_heap_valid with "Hσ Hl") as %?.
+  iSplit.
+  inv_head_step.
+  admit.
+  iIntros (κ v2 σ2 efs Hstep); inv_head_step.
+  move: H1 => [H1 H2].
+  iModIntro; iSplit=> //; iSplit=> //.
+  iSplitR.
+  admit.
+  unfold from_option.
+  inversion H0 => {H0}; subst.
+  { inversion H3 => {H3}; subst.
+    { exfalso.
+      admit. }
+    { exfalso.
+      admit. }
+    { simpl.
+      clear H0.
+      apply lfilled_Ind_Equivalent in H1.
+      inversion H1; subst.
+      { admit. }
+    }
+  }
+  { simpl.
+    exfalso.
+    move: H3.
+    rewrite app_singleton => H3.
+    move: H3 => [[H3 H4]|[H3 H4]]; discriminate. }
+  { admit. }
+  { admit. }
+  { exfalso.
+  move: H3.
+  rewrite app_nil => [[_ H4]].
+  discriminate. }
+Admitted.
+
+Lemma twp_wp_step s E e P Φ :
+  TCEq (to_val e) None →
+  ▷ P -∗
+  WP e @ s; E [{ v, P ={E}=∗ Φ v }] -∗ WP e @ s; E {{ Φ }}.
+Proof.
+  iIntros (?) "HP Hwp".
+  iApply (wp_step_fupd _ _ E _ P with "[HP]"); [auto..|].
+  { by inversion H; subst. }
+  by iApply twp_wp.
+Qed.
+
+Lemma wp_load s E imm q v :
+  {{{ ▷ locof imm ↦{q} v }}} [Basic (Get_local imm)] @ s; E {{{ RET v; locof imm ↦{q} v }}}.
+Proof.
+  iIntros (Φ) ">H HΦ". iApply (twp_wp_step with "HΦ").
+  iApply (twp_load with "H"); [auto..|]; iIntros "H HΦ". by iApply "HΦ".
+Qed.
+
+End lifting.
+*)
 
